done/Iron/Language/SystemF2Effect/Type/Relation/WfT.v
@@ -54,9 +54,9 @@ Notation ClosedT := (WfT 0).
 
 (******************************************************************************)
 Lemma closedT_tRef
- :  forall r1 t2
+ :  forall p1 t2
  ,  ClosedT t2
- -> ClosedT (TRef (TRgn r1) t2).
+ -> ClosedT (TRef (TRgn p1) t2).
 Proof. auto. Qed.
 Hint Resolve closedT_tRef.
 
